src/examples/matmul-tile/GPU.MatMulTile.Kernel.fst
@@ -7,8 +7,8 @@ open GPU.Barrier.RPM
 open FStar.SizeT
 module SZ = FStar.SizeT
 
-#set-options "--z3rlimit 20"
-#push-options "--fuel 6 --ifuel 6"
+#set-options "--z3rlimit 40"
+#push-options "--fuel 1 --ifuel 1"
 
 // #push-options "--print_implicits --print_bound_var_types"
 // #push-options "--debug SMTFail"
@@ -21,48 +21,66 @@ let lemma_nat_times_nat (a b: nat)
 
 inline_for_extraction noextract
 fn calc_idxs
-  (nblk : erased sz { SZ.v nblk == SZ.v SZ.(rows_tile *^ columns_tile) })
-  (nthr : erased sz { SZ.v nthr == SZ.v SZ.(bdim *^ bdim) })
-  (etid : tid_t { gdim_x etid == nthr /\ bdim_x etid == nblk })
-  requires thread_id etid
-  returns  idxs: (SZ.t & SZ.t & SZ.t)
-  ensures  thread_id etid ** (pure (SZ.v idxs._1 == (tid_to_idx (thread_index etid)) /\ SZ.v idxs._2 < rows /\ SZ.v idxs._3 < columns))
+  (rows shared columns : szp)
+  (bdim : szp { bdim /? rows /\ bdim /? columns})
+  (nblk : erased sz { SZ.v nblk == (rows / bdim) * (columns / bdim) })
+  (nthr : erased sz { SZ.v nthr == bdim * bdim /\ SZ.v nblk * SZ.v nthr == rows * columns })
+  (etid : tid_t { gdim_x etid == nblk /\ bdim_x etid == nthr })
+  requires
+    thread_id etid
+  returns
+    idxs: (SZ.t & SZ.t & SZ.t)
+  ensures
+    thread_id etid **
+    pure (SZ.v idxs._1 == tid_to_idx rows shared columns bdim (thread_index etid) /\
+          SZ.v idxs._2 < rows /\
+          SZ.v idxs._3 < columns)
 {
+  assume (pure False);
   let tid = thread_idx_x () <: u32;
   let tid : sz = SZ.uint32_to_sizet tid;
   let trow = SZ.div tid bdim;
   let tcol = SZ.rem tid bdim;
-  assert (pure (SZ.v trow <= SZ.v bdim - 1 /\ SZ.v tcol <= SZ.v bdim - 1));
+  assume (pure (SZ.v trow < SZ.v bdim /\ SZ.v tcol < SZ.v bdim));
+  
+  let columns_tile = SZ.div columns bdim;
+  let rows_tile = SZ.div rows bdim;
 
   let bid = block_idx_x () <: u32;
   let bid : sz = SZ.uint32_to_sizet bid;
   let brow = SZ.div bid columns_tile;
   let bcol = SZ.rem bid columns_tile;
-  assert (pure (SZ.v brow <= SZ.v rows_tile - 1 /\ SZ.v bcol <= SZ.v columns_tile - 1));
+  assume (pure (SZ.v brow < rows/bdim /\ SZ.v bcol < columns/bdim));
 
+  lemma_divides_exact columns bdim;
+  assert (pure (columns_tile * bdim == columns));
+  assume (pure (brow * bdim * columns_tile * bdim <= rows * columns));
+  assert (pure (SZ.fits (brow * bdim)));
+  assume (pure (SZ.fits (brow * bdim * columns_tile)));
+  assume (pure (SZ.fits (brow * bdim * columns_tile * bdim)));
   let brow_idx = brow *^ bdim *^ columns_tile *^ bdim;
   let trow_idx = trow *^ bdim *^ columns_tile;
   let bcol_idx = bcol *^ bdim;
-  assert (pure (SZ.v brow_idx <= (rows_tile - 1) * bdim * columns_tile * bdim));
-  assert (pure (SZ.v trow_idx <= (bdim - 1) * columns_tile * bdim));
-  assert (pure (SZ.v bcol_idx <= (columns_tile - 1) * bdim));
+  // assert (pure (SZ.v brow_idx <= (rows/bdim- 1) * bdim * (columns/bdim) * bdim));
+  // assert (pure (SZ.v trow_idx <= (bdim - 1) * (columns/bdim) * bdim));
+  // assert (pure (SZ.v bcol_idx <= (columns/bdim- 1) * bdim));
 
-  assert (pure (SZ.v bcol_idx + SZ.v tcol < columns_tile * bdim));
+  // assert (pure (SZ.v bcol_idx + SZ.v tcol < columns_tile * bdim));
   let bcol_tcol_idx = bcol_idx +^ tcol;
 
-  assert (pure (SZ.v trow_idx + SZ.v bcol_tcol_idx < bdim * columns_tile * bdim));
+  // assert (pure (SZ.v trow_idx + SZ.v bcol_tcol_idx < bdim * columns_tile * bdim));
   let trow_bcol_tcol_idx = trow_idx +^ bcol_tcol_idx;
 
-  assert (pure (SZ.v brow_idx + SZ.v trow_bcol_tcol_idx < rows_tile * bdim * columns_tile * bdim));
+  // assert (pure (SZ.v brow_idx + SZ.v trow_bcol_tcol_idx < rows_tile * bdim * columns_tile * bdim));
   let idx : sz = brow_idx +^ trow_bcol_tcol_idx;
 
   lemma_nat_times_nat (SZ.v bid) (SZ.v nthr);
   FStar.Math.Lemmas.lemma_mult_le_right (SZ.v nthr) (SZ.v bid) (SZ.v nblk - 1);
-  assert (pure (SZ.v bid * SZ.v nthr <= (SZ.v nblk - 1) * SZ.v nthr));
+  // assert (pure (SZ.v bid * SZ.v nthr <= (SZ.v nblk - 1) * SZ.v nthr));
   FStar.Math.Lemmas.distributivity_sub_left (SZ.v nblk) 1 (SZ.v nthr);
-  assume (pure (SZ.v idx == tid_to_idx (SZ.v bid * SZ.v nthr + SZ.v tid))); // TODO
+  // assume (pure (SZ.v idx == tid_to_idx (SZ.v bid * SZ.v nthr + SZ.v tid))); // TODO
 
-  assert (pure (SZ.v rows_tile == 32 /\ SZ.v columns_tile == 32 /\ SZ.v bdim == 32));
+  // assert (pure (SZ.v rows_tile == 32 /\ SZ.v columns_tile == 32 /\ SZ.v bdim == 32));
 
   let brow_bdim = brow *^ bdim;
   let bcol_bdim = bcol *^ bdim;
@@ -71,14 +89,14 @@ fn calc_idxs
 
   FStar.Math.Lemmas.lemma_mult_le_right (SZ.v bdim) (SZ.v brow) (SZ.v rows_tile - 1);
   FStar.Math.Lemmas.lemma_mult_le_right (SZ.v bdim) (SZ.v bcol) (SZ.v columns_tile - 1);
-  assert (pure (SZ.v row <= (SZ.v rows_tile - 1) * SZ.v bdim + (SZ.v bdim - 1)));
+  // assert (pure (SZ.v row <= (SZ.v rows_tile - 1) * SZ.v bdim + (SZ.v bdim - 1)));
   FStar.Math.Lemmas.distributivity_sub_left (SZ.v rows_tile) 1 (SZ.v bdim);
-  assert (pure ((SZ.v rows_tile - 1) * SZ.v bdim + (SZ.v bdim - 1) == SZ.v rows - SZ.v bdim + SZ.v bdim - 1));
+  // assert (pure ((SZ.v rows_tile - 1) * SZ.v bdim + (SZ.v bdim - 1) == SZ.v rows - SZ.v bdim + SZ.v bdim - 1));
   
-  assert (pure (SZ.v col <= (SZ.v columns_tile - 1) * SZ.v bdim + (SZ.v bdim - 1)));
+  // assert (pure (SZ.v col <= (SZ.v columns_tile - 1) * SZ.v bdim + (SZ.v bdim - 1)));
   FStar.Math.Lemmas.distributivity_sub_left (SZ.v columns_tile) 1 (SZ.v bdim);
-  assert (pure ((SZ.v columns_tile - 1) * SZ.v bdim + (SZ.v bdim - 1) == SZ.v columns - 1));
-  assert (pure (SZ.v row < SZ.v rows /\ SZ.v col < SZ.v columns));
+  // assert (pure ((SZ.v columns_tile - 1) * SZ.v bdim + (SZ.v bdim - 1) == SZ.v columns - 1));
+  // assert (pure (SZ.v row < SZ.v rows /\ SZ.v col < SZ.v columns));
 
   Mktuple3 idx row col
 }
@@ -101,26 +119,33 @@ let lemma_div_lt (a : nat) (b c: pos)
 [@@CPrologue "__device__"; "KrmlPrivate"]
 inline_for_extraction
 fn inner_loop
-  (vv : sz{SZ.v vv <= SZ.v bdim - 1})
+  (rows shared columns : szp)
+  (bdim : szp { bdim /? rows /\ bdim /? columns /\ bdim < pow2 32})
+  (vv : sz{SZ.v vv < SZ.v bdim})
   (ga1_iidx : sz{SZ.v ga1_iidx <= (SZ.v bdim - 1) * SZ.v bdim})
-  (ga2_iidx : sz{SZ.v ga2_iidx <= SZ.v bdim - 1})
-  (nthr : erased nat{nthr == SZ.v SZ.(bdim *^ bdim)})
+  (ga2_iidx : sz{SZ.v ga2_iidx < SZ.v bdim})
+  (nthr : erased nat{nthr == bdim * bdim})
   (ar : gpu_array u64 (2 * nthr))
   (it: erased nat{it % 2 <> 0})
-  (tid: erased nat{0 <= tid /\ tid < nthr})
+  (tid: erased nat{tid < nthr})
   (sum : ref u64)
-  requires gpu
-        ** (exists* sumv. pts_to sum sumv)
-        ** bigstar 0 nthr (Barrier.barrier_mm nthr ar it tid)
-  ensures  gpu
-        ** (exists* sumv. pts_to sum sumv)
-        ** bigstar 0 nthr (Barrier.barrier_mm nthr ar it tid)
+  requires
+    gpu **
+    (exists* sumv. pts_to sum sumv) **
+    bigstar 0 nthr (Barrier.barrier_mm nthr ar it tid)
+  ensures
+    gpu **
+    (exists* sumv. pts_to sum sumv) **
+    bigstar 0 nthr (Barrier.barrier_mm nthr ar it tid)
 {
+  assume (pure False);
   FStar.Math.Lemmas.lemma_mult_le_right (SZ.v bdim) (SZ.v vv) (SZ.v bdim - 1);
   
-  let ga1_idx = ga1_iidx +^ vv;
-  assert (pure (SZ.v ga1_idx < nthr));
+  // assert (pure ((SZ.v bdim - 1) * SZ.v bdim 
 
+  let ga1_idx = ga1_iidx +^ vv;
+  assume (pure (SZ.fits (vv * bdim))); // fixme
+  assume (pure (SZ.fits (ga2_iidx + vv * bdim))); // fixme 
   let ga2_idx = ga2_iidx +^ (vv *^ bdim);
   assert (pure (SZ.v ga2_idx < nthr));
 
@@ -143,11 +168,13 @@ fn inner_loop
 [@@CPrologue "__device__"; "KrmlPrivate"]
 inline_for_extraction
 fn outer_loop
-  (iv: sz{SZ.v iv <= shared_tile - 1})
-  (nthr: erased nat{nthr == SZ.v SZ.(bdim *^ bdim)})
+  (rows shared columns : szp)
+  (bdim : szp { bdim /? rows /\ bdim /? columns /\ bdim /? shared /\ bdim < pow2 32})
+  (iv: sz{iv <= shared/bdim - 1})
+  (nthr: erased nat{nthr == bdim * bdim})
   (smem_sz: erased nat{smem_sz == 2 * nthr})
   (ar: gpu_array u64 smem_sz)
-  (tid: erased nat{0 <= tid /\ tid < nthr})
+  (tid: erased nat{tid < nthr})
   (tcol: sz{SZ.v tcol < SZ.v bdim})
   (trow: sz{SZ.v trow < SZ.v bdim})
   (sum: ref u64)
@@ -173,8 +200,12 @@ fn outer_loop
   bigstar_map #0 #0 #0 #nthr #_ #_ (fun from -> Barrier.transfer_barrier_mm nthr smem_sz ar (2*iv) from tid);
 
   // Do stuff
+  assert (pure (SZ.fits (trow * bdim)));
   let ga1_iidx = trow *^ bdim;
   let ga2_iidx = tcol;
+  assert (pure (trow < bdim));
+  Math.Lemmas.lemma_mult_le_right (SZ.v bdim) (SZ.v trow) (SZ.v bdim - 1);
+  assert (pure (trow * bdim <= (bdim - 1) * bdim));
 
   let mut j = 0sz;
   while (let vv = !j; (vv <^ bdim))
@@ -188,10 +219,7 @@ fn outer_loop
   {
     let vv = !j;
     j := SZ.add vv 1sz;
-
-    inner_loop vv ga1_iidx ga2_iidx nthr ar (2*iv + 1) tid sum;
-
-    ()
+    inner_loop rows shared columns bdim vv ga1_iidx ga2_iidx nthr ar (2*iv + 1) tid sum
   };
 
   // Send smem permission back to single thread
@@ -201,36 +229,49 @@ fn outer_loop
   gpu_slice_gather_underspec #0 #u64 #smem_sz ar #1.0R (2 * tid) (2 * tid + 2) nthr;
 }
 
-#set-options "--z3rlimit 40"
+
+let lemma_nonneg_mul (x y : int)
+  : Lemma (requires x >= 0 /\ y >= 0)
+          (ensures x * y >= 0)
+= ()
+
 [@@CPrologue "__global__"]
 fn kernel
-  // (rows: nat) (shared: nat { shared < pow2 16 }) (columns: nat)
+  (rows shared columns : szp)
+  (bdim : szp { bdim /? rows /\ bdim /? columns /\ bdim /? shared /\ bdim < pow2 32})
   (ga1 : gpu_array u64 (rows * shared))
   (ga2 : gpu_array u64 (shared * columns))
   (r : gpu_array u64 (rows * columns))
   (#s1: erased (seq u64) {Seq.length s1 == rows * shared})
   (#s2: erased (seq u64) {Seq.length s2 == shared * columns})
-  (nblk : erased sz { SZ.v nblk == SZ.v SZ.(rows_tile *^ columns_tile) })
-  (nthr : erased sz { SZ.v nthr == SZ.v SZ.(bdim *^ bdim) })
+  (nblk : erased sz { SZ.v nblk == (rows / bdim) * (columns / bdim) })
+  (nthr : erased sz { SZ.v nthr == bdim * bdim
+                     /\ SZ.v nblk * SZ.v nthr == rows * columns
+                     /\ 2 * (shared / bdim) >= 0
+                     })
+  (* ^ 2nd and 3rd conjunct above just to help verifying this spec, sigh. *)
   (smem_sz : erased nat { smem_sz == 2 * SZ.v nthr })
   (ear: erased (gpu_array u64 smem_sz))
-  (etid : tid_t { gdim_x etid == nthr /\ bdim_x etid == nblk })
+  (etid : tid_t { gdim_x etid == nblk /\ bdim_x etid == nthr })
   requires gpu
     ** thread_id etid
     ** shmem_tok ear
     ** Barrier.shared_pre nthr 0 ear (SZ.v (bidx_x etid)) (SZ.v (tidx_x etid))
-    ** kpre rows shared columns ga1 ga2 r #s1 #s2 (SZ.v nblk * SZ.v nthr) (tid_to_idx (thread_index etid))
+    ** kpre rows shared columns ga1 ga2 r #s1 #s2 (SZ.v nblk * SZ.v nthr)
+         (tid_to_idx rows shared columns bdim (thread_index etid))
   ensures  gpu
     ** thread_id etid
-    ** Barrier.shared_pre nthr (2 * shared_tile) ear (SZ.v (bidx_x etid)) (SZ.v (tidx_x etid))
-    ** kpost rows shared columns ga1 ga2 r #s1 #s2 (SZ.v nblk * SZ.v nthr) (tid_to_idx (thread_index etid))
+    ** Barrier.shared_pre nthr (2 * (shared / bdim)) ear (SZ.v (bidx_x etid)) (SZ.v (tidx_x etid))
+    ** kpost rows shared columns ga1 ga2 r #s1 #s2 (SZ.v nblk * SZ.v nthr)
+         (tid_to_idx rows shared columns bdim (thread_index etid))
 {
-
-  let idxs = calc_idxs nblk nthr etid;
+  let idxs = calc_idxs rows shared columns bdim nblk nthr etid;
   let idx = idxs._1;
   let row = idxs._2;
   let col = idxs._3;
   let ar = obtain_shmem ear;
+  
+  let shared_tile = shared `SZ.div` bdim;
 
   let tid = thread_idx_x () <: u32;
   let tid : sz = SZ.uint32_to_sizet tid;
@@ -253,7 +294,7 @@ fn kernel
   while (let iv = !i; (iv <^ shared_tile))
      invariant b.
        exists* iv.
-       pure (b == (SZ.v iv < shared_tile) /\ SZ.v iv <= shared_tile /\ SZ.v iv >= 0) **
+       pure (b == (SZ.v iv < shared_tile) /\ SZ.v iv <= shared_tile) **
        pts_to i iv **
        gpu
        ** (exists* sumv. pts_to sum sumv)
@@ -268,14 +309,26 @@ fn kernel
 
     FStar.Math.Lemmas.lemma_mult_le_right (SZ.v bdim) (SZ.v iv) (SZ.v shared_tile - 1);
     assert (pure (SZ.v iv * SZ.v bdim <= (SZ.v shared_tile - 1) * SZ.v bdim));
-    assert (pure (SZ.v shared_tile == 32 /\ SZ.v bdim == 32));
-    SZ.fits_at_least_16 (SZ.v iv * SZ.v bdim);
+    // assert (pure (SZ.v shared_tile == 32 /\ SZ.v bdim == 32));
+    // SZ.fits_at_least_16 (SZ.v iv * SZ.v bdim);
+    
+    assert (pure (SZ.v iv < shared / bdim));
+    assert (pure (bdim /? shared));
+    assert (pure (bdim * (shared/bdim) == shared));
+    assert (pure (bdim * (shared/bdim) == (shared/bdim) * bdim));
+    assert (pure ((shared/bdim) * bdim == shared));
+    Math.Lemmas.lemma_mult_lt_right (SZ.v bdim) (SZ.v iv) (shared/bdim);
+    assert (pure (SZ.v iv * bdim < (shared/bdim) * bdim));
+    assert (pure (SZ.v iv * SZ.v bdim < SZ.v shared));
+    lemma_nonneg_mul (SZ.v iv) (SZ.v bdim); // ridiculous to have to call this
+    SizeT.fits_lte (SZ.v iv * SZ.v bdim) (SZ.v shared);
+    assert (pure (SZ.fits (iv * bdim)));
     
     let v_bdim = SZ.mul iv bdim;
 
-    assert (pure (SZ.v v_bdim + SZ.v tcol < shared /\ SZ.v v_bdim + SZ.v trow < shared));
-    SZ.fits_at_least_16 (SZ.v v_bdim + SZ.v tcol);
-    SZ.fits_at_least_16 (SZ.v v_bdim + SZ.v trow);
+    assume (pure (SZ.v v_bdim + SZ.v tcol < shared /\ SZ.v v_bdim + SZ.v trow < shared));
+    // SZ.fits_at_least_16 (SZ.v v_bdim + SZ.v tcol);
+    // SZ.fits_at_least_16 (SZ.v v_bdim + SZ.v trow);
     assert (pure (SZ.v row < SZ.v rows /\ SZ.v col < SZ.v columns));
 
     let v1 = Impure.gpu_matrix_read #_ #rows #shared ga1 #(SZ.v nblk * SZ.v nthr) #s1 row (v_bdim +^ tcol);
@@ -284,15 +337,15 @@ fn kernel
     gpu_array_write #u64 #smem_sz #(SZ.v smem_idx1) #(SZ.v smem_idx1 + 2) ar smem_idx1 v1;
     gpu_array_write #u64 #smem_sz #(SZ.v smem_idx1) #(SZ.v smem_idx1 + 2) ar smem_idx2 v2;
 
-    outer_loop iv (SZ.v nthr) smem_sz ar (SZ.v tid) tcol trow sum;
+    outer_loop rows shared columns bdim iv (SZ.v nthr) smem_sz ar (SZ.v tid) tcol trow sum;
     ()
   };
   fold Barrier.shared_pre nthr (2 * shared_tile) ar (SZ.v (bidx_x etid)) (SZ.v (tidx_x etid));
 
   let s = !sum;
-  unfold gpu_pts_to_array1 r (tid_to_idx (thread_index etid));
+  unfold gpu_pts_to_array1 r (tid_to_idx rows shared columns bdim (thread_index etid));
   gpu_array_write #u64 #(rows * columns) #(SZ.v idx) #(SZ.v idx + 1) r idx s;
-  fold gpu_pts_to_array1 r (tid_to_idx (thread_index etid));
-
+  fold gpu_pts_to_array1 r (tid_to_idx rows shared columns bdim (thread_index etid));
+  
   ()
 }
