src/examples/matmul-tile/GPU.MatMulTile.fst
@@ -1,9 +1,10 @@
 module GPU.MatMulTile
 #lang-pulse
 
-#push-options "--fuel 1 --ifuel 1"
+#set-options "--fuel 1 --ifuel 1 --z3rlimit 40"
 
 open GPU
+open GPU.Math
 
 module A    = Pulse.Lib.Array
 module SZ   = FStar.SizeT
@@ -11,92 +12,133 @@ module Defs = GPU.MatMul.Defs
 module Kernel = GPU.MatMulTile.Kernel
 module Barrier = GPU.MatMulTile.Barrier
 
+let lemma_nonneg_mul (x y : int)
+  : Lemma (requires x >= 0 /\ y >= 0)
+          (ensures x * y >= 0)
+= ()
+
 ghost
 fn setup
-  (nblk: sz { nblk == SZ.(Kernel.rows_tile *^ Kernel.columns_tile) })
-  (nthr: sz { nthr == SZ.(Kernel.bdim *^ Kernel.bdim) })
-  (ga1 : gpu_array u64 (Kernel.rows * Kernel.shared))
-  (ga2 : gpu_array u64 (Kernel.shared * Kernel.columns))
-  (gr  : gpu_array u64 (nblk * nthr))
-  (v1: erased (seq u64) { Seq.length v1 == Kernel.rows * Kernel.shared })
-  (v2: erased (seq u64) { Seq.length v2 == Kernel.shared * Kernel.columns })
+  (rows shared columns : szp)
+  (bdim : szp { bdim /? rows /\ bdim /? columns /\ bdim /? shared /\ bdim < pow2 32})
+  (nblk : erased sz { SZ.v nblk == (rows / bdim) * (columns / bdim) })
+  (nthr : erased sz { SZ.v nthr == bdim * bdim
+                     /\ SZ.v nblk * SZ.v nthr == rows * columns
+                     /\ 2 * (shared / bdim) >= 0
+                     })
+  (* ^ 2nd and 3rd conjunct above just to help verifying this spec, sigh. *)
+  (ga1 : gpu_array u64 (rows * shared))
+  (ga2 : gpu_array u64 (shared * columns))
+  (gr  : gpu_array u64 (SZ.v nblk * SZ.v nthr))
+  (v1: erased (seq u64) { Seq.length v1 == rows * shared })
+  (v2: erased (seq u64) { Seq.length v2 == shared * columns })
   requires gpu_pts_to_array gr 's **
            gpu_pts_to_array ga1 v1 **
            gpu_pts_to_array ga2 v2
-  ensures  bigstar 0 (nblk * nthr) (fun i ->
-             Kernel.kpre Kernel.rows Kernel.shared Kernel.columns ga1 ga2 gr #v1 #v2 (nblk * nthr) (Kernel.tid_to_idx i))
+  ensures  bigstar 0 (SZ.v nblk * SZ.v nthr) (fun i ->
+             Kernel.kpre rows shared columns ga1 ga2 gr #v1 #v2 (SZ.v nblk * SZ.v nthr)
+               (Kernel.tid_to_idx rows shared columns bdim i))
 {
   // Sharing the input matrices (splitting permissions)
-  fold Defs.gpu_pts_to_matrix Kernel.rows   Kernel.shared  ga1 1 v1;
-  fold Defs.gpu_pts_to_matrix Kernel.shared Kernel.columns ga2 1 v2;
-  Defs.gpu_matrix_share_underspec #_ #1 Kernel.rows   Kernel.shared  ga1 (nblk * nthr) v1;
-  Defs.gpu_matrix_share_underspec #_ #2 Kernel.shared Kernel.columns ga2 (nblk * nthr) v2;
+  fold Defs.gpu_pts_to_matrix rows   shared  ga1 1 v1;
+  fold Defs.gpu_pts_to_matrix shared columns ga2 1 v2;
+  Defs.gpu_matrix_share_underspec #_ #1 rows   shared  ga1 (SZ.v nblk * SZ.v nthr) v1;
+  Defs.gpu_matrix_share_underspec #_ #2 shared columns ga2 (SZ.v nblk * SZ.v nthr) v2;
 
   // Sharing the output matrix (splitting each cell)
   gpu_pts_to_ref gr; (* obtain length v == (nblk * nthr) *)
   gpu_array_slice_1 #4 gr;
 
   // Join resources into a single bigstar
-  bigstar_zip #1 #2 #3 0 (nblk * nthr) _ _;
-  bigstar_zip #3 #4 #0 0 (nblk * nthr) _ _;
+  bigstar_zip #1 #2 #3 0 (SZ.v nblk * SZ.v nthr) _ _;
+  bigstar_zip #3 #4 #0 0 (SZ.v nblk * SZ.v nthr) _ _;
 
   // Rewrite inside the bigstar
   ghost
-  fn aux (i:nat{0 <= i /\ i < (nblk * nthr)})
+  fn aux (i:nat{0 <= i /\ i < (SZ.v nblk * SZ.v nthr)})
     requires
-      Defs.gpu_pts_to_matrix Kernel.rows   Kernel.shared  ga1 (nblk * nthr) v1 **
-      Defs.gpu_pts_to_matrix Kernel.shared Kernel.columns ga2 (nblk * nthr) v2 **
+      Defs.gpu_pts_to_matrix rows   shared  ga1 (SZ.v nblk * SZ.v nthr) v1 **
+      Defs.gpu_pts_to_matrix shared columns ga2 (SZ.v nblk * SZ.v nthr) v2 **
       gpu_pts_to_array_slice gr i (i + 1) seq!['s `Seq.index` i]
     ensures
-      Kernel.kpre Kernel.rows Kernel.shared Kernel.columns ga1 ga2 gr #v1 #v2 (nblk * nthr) i
+      Kernel.kpre rows shared columns ga1 ga2 gr #v1 #v2 (SZ.v nblk * SZ.v nthr) i
   {
     fold gpu_pts_to_array1 gr i;
     ()
   };
-  bigstar_map #_ #_ #0 #(nblk * nthr) aux;
-  bigstar_permute #0 #0 #(nblk * nthr) #_ (Kernel.permute());
-  ghost fn rewrite_permute_to_fn (i: nat {0 <= i /\ i < (nblk * nthr)})
-    requires Kernel.kpre Kernel.rows Kernel.shared Kernel.columns ga1 ga2 gr #v1 #v2 (nblk * nthr) ((Kernel.permute()).f i)
-    ensures  Kernel.kpre Kernel.rows Kernel.shared Kernel.columns ga1 ga2 gr #v1 #v2 (nblk * nthr) (Kernel.tid_to_idx i)
+  let _ = calc (==) {
+    (rows / bdim) * (columns / bdim) * bdim * bdim;
+    == { magic() } // fixme, boring proof (we have divisibility)
+    rows * columns;
+  };
+  bigstar_map #_ #_ #0 #(SZ.v nblk * SZ.v nthr) aux;
+  lemma_nonneg_mul (SZ.v nblk) (SZ.v nthr);
+  lemma_divides_exact rows bdim;
+  lemma_divides_exact columns bdim;
+  assert (pure (rows / bdim >= 1));
+  assert (pure (columns / bdim >= 1));
+  bigstar_permute #0 #0 #(SZ.v nblk * SZ.v nthr) #_ (Kernel.permute (rows/bdim) (columns/bdim) bdim);
+  ghost fn rewrite_permute_to_fn (i: nat {0 <= i /\ i < (SZ.v nblk * SZ.v nthr)})
+    requires Kernel.kpre rows shared columns ga1 ga2 gr #v1 #v2 (SZ.v nblk * SZ.v nthr) ((Kernel.permute (rows/bdim) (columns/bdim) bdim).f i)
+    ensures  Kernel.kpre rows shared columns ga1 ga2 gr #v1 #v2 (SZ.v nblk * SZ.v nthr) (Kernel.tid_to_idx rows shared columns bdim i)
   {
     ()
   };
-  bigstar_map #0 #0 #0 #(nblk * nthr) (fun i -> rewrite_permute_to_fn i);
+  bigstar_map #0 #0 #0 #(SZ.v nblk * SZ.v nthr) (fun i -> rewrite_permute_to_fn i);
   ()
 }
 
 ghost
 fn breakdown
-  (nblk: sz { nblk == SZ.(Kernel.rows_tile *^ Kernel.columns_tile) })
-  (nthr: sz { nthr == SZ.(Kernel.bdim *^ Kernel.bdim) })
-  (ga1 : gpu_array u64 (Kernel.rows * Kernel.shared))
-  (ga2 : gpu_array u64 (Kernel.shared * Kernel.columns))
+  (rows shared columns : szp)
+  (bdim : szp { bdim /? rows /\ bdim /? columns /\ bdim /? shared /\ bdim < pow2 32})
+  (nblk : sz { SZ.v nblk == (rows / bdim) * (columns / bdim) })
+  (nthr : sz { SZ.v nthr == bdim * bdim
+                     /\ SZ.v nblk * SZ.v nthr == rows * columns
+                     /\ 2 * (shared / bdim) >= 0
+                     })
+  (* ^ 2nd and 3rd conjunct above just to help verifying this spec, sigh. *)
+  (ga1 : gpu_array u64 (rows * shared))
+  (ga2 : gpu_array u64 (shared * columns))
   (gr  : gpu_array u64 (nblk * nthr))
-  (v1: erased (seq u64) { Seq.length v1 == Kernel.rows * Kernel.shared })
-  (v2: erased (seq u64) { Seq.length v2 == Kernel.shared * Kernel.columns })
-  requires bigstar 0 (nblk * nthr) (fun i ->
-             Kernel.kpost Kernel.rows Kernel.shared Kernel.columns ga1 ga2 gr #v1 #v2 (nblk * nthr) (Kernel.tid_to_idx i))
-  ensures  (exists* vr. gpu_pts_to_array gr vr) **
-           gpu_pts_to_array ga1 v1 **
-           gpu_pts_to_array ga2 v2
+  (v1: erased (seq u64) { Seq.length v1 == rows * shared })
+  (v2: erased (seq u64) { Seq.length v2 == shared * columns })
+  requires
+    bigstar 0 (nblk * nthr) (fun i ->
+      Kernel.kpost rows shared columns ga1 ga2 gr #v1 #v2 (nblk * nthr) (Kernel.tid_to_idx rows shared columns bdim i))
+  ensures
+    (exists* vr. gpu_pts_to_array gr vr) **
+    gpu_pts_to_array ga1 v1 **
+    gpu_pts_to_array ga2 v2
 {
-  let perm = perm_inv (Kernel.permute());
+  lemma_nonneg_mul (SZ.v nblk) (SZ.v nthr);
+  lemma_divides_exact rows bdim;
+  lemma_divides_exact columns bdim;
+  let _ = calc (==) {
+    (rows / bdim) * (columns / bdim) * bdim * bdim;
+    == { magic() } // fixme, boring proof (we have divisibility)
+    rows * columns;
+  };
+  assert (pure (rows / bdim >= 1));
+  assert (pure (columns / bdim >= 1));
+  let perm = perm_inv (Kernel.permute (rows/bdim) (columns/bdim) bdim);
   bigstar_permute #0 #0 #(nblk * nthr) #_ perm;
   ghost fn rewrite_permute_to_fn (i: nat {0 <= i /\ i < (nblk * nthr)})
-    requires Kernel.kpost Kernel.rows Kernel.shared Kernel.columns ga1 ga2 gr #v1 #v2 (nblk * nthr) (perm.f (Kernel.tid_to_idx i))
-    ensures  Kernel.kpost Kernel.rows Kernel.shared Kernel.columns ga1 ga2 gr #v1 #v2 (nblk * nthr) i
+    requires Kernel.kpost rows shared columns ga1 ga2 gr #v1 #v2 (nblk * nthr) (perm.f (Kernel.tid_to_idx rows shared columns bdim i))
+    ensures  Kernel.kpost rows shared columns ga1 ga2 gr #v1 #v2 (nblk * nthr) i
   {
-    let once: (j: nat{ 0 <= j /\ j < (nblk * nthr) }) = Kernel.tid_to_idx i;
+    let once: (j: nat{ 0 <= j /\ j < (nblk * nthr) }) = Kernel.tid_to_idx rows shared columns bdim i;
     let once': (j: nat{ 0 <= j /\ j < (nblk * nthr) }) = perm.g i;
     assert (pure (once' == once));
     perm.proof once i;
     // f x == y <==> g y == x
     let double: (j: nat{ 0 <= j /\ j < (nblk * nthr) }) = perm.f once;
     assert (pure (double == i));
-    rewrite (gpu_pts_to_array1 gr (perm.f (Kernel.tid_to_idx i)))
+    rewrite (gpu_pts_to_array1 gr (perm.f (Kernel.tid_to_idx rows shared columns bdim i)))
          as (gpu_pts_to_array1 gr i);
     ()
   };
+  admit();
   bigstar_map #0 #0 #0 #(nblk * nthr) (fun i -> rewrite_permute_to_fn i);
 
   // Join resources into a single bigstar
@@ -106,52 +148,107 @@ fn breakdown
   gpu_array_unslice_1_underspec #4 gr #1.0R;
 
   // Unsharing the input matrices (gathering permissions)
-  Defs.gpu_matrix_unshare_underspec #_ #1 Kernel.rows   Kernel.shared  ga1 (nblk * nthr) v1;
-  Defs.gpu_matrix_unshare_underspec #_ #2 Kernel.shared Kernel.columns ga2 (nblk * nthr) v2;
-  unfold Defs.gpu_pts_to_matrix Kernel.rows   Kernel.shared  ga1 1 v1;
-  unfold Defs.gpu_pts_to_matrix Kernel.shared Kernel.columns ga2 1 v2;
+  Defs.gpu_matrix_unshare_underspec #_ #1 rows   shared  ga1 (nblk * nthr) v1;
+  Defs.gpu_matrix_unshare_underspec #_ #2 shared columns ga2 (nblk * nthr) v2;
+  unfold Defs.gpu_pts_to_matrix rows   shared  ga1 1 v1;
+  unfold Defs.gpu_pts_to_matrix shared columns ga2 1 v2;
 
   ()
 }
 
+let stupid_mul_mono (x y z w : nat)
+: Lemma (requires x <= z /\ y <= w) (ensures x * y <= z * w)
+=
+  ()
+
+let stupid_divides (x:nat) (y:pos)
+: Lemma (x/y <= x)
+  [SMTPat (x/y)]
+=
+  admit() // prove
+
+#set-options "--z3rlimit 20"
 fn main
+  (rows shared columns : szp)
+  (bdim : szp { bdim /? rows /\ bdim /? columns /\ bdim /? shared /\ bdim < pow2 30})
   (a1 a2: array u64)
-  (v1: erased (seq u64) { Seq.length v1 == Kernel.rows * Kernel.shared })
-  (v2: erased (seq u64) { Seq.length v2 == Kernel.shared * Kernel.columns })
-  requires cpu ** A.pts_to a1 v1 ** A.pts_to a2 v2
+  (v1: erased (seq u64) { Seq.length v1 == rows * shared })
+  (v2: erased (seq u64) { Seq.length v2 == shared * columns })
+  requires
+    cpu **
+    A.pts_to a1 v1 **
+    A.pts_to a2 v2 **
+    pure (SZ.fits (rows * columns) /\ SZ.fits (rows * shared) /\ SZ.fits (shared * columns))
   returns  ar: array u64
   ensures  cpu ** A.pts_to a1 v1 ** A.pts_to a2 v2 ** (exists* vr. A.pts_to ar vr)
 {
   open FStar.SizeT;
-  let nblk = Kernel.rows_tile *^ Kernel.columns_tile;
-  let nthr = Kernel.bdim *^ Kernel.bdim;
+  let rows_tile = div rows bdim;
+  let columns_tile = SZ.div columns bdim;
+  mul_pow2 30 30; // sigh
+  assert (pure (pow2 30 * pow2 30 == pow2 60));
+  assert (pure (rows_tile <= rows));
+  assert (pure (columns_tile <= columns));
+  assert (pure (SZ.fits (rows * columns)));
+  stupid_mul_mono rows_tile columns_tile rows columns;
+  assert (pure (rows_tile * columns_tile <= rows * columns));
+  assert (pure (SZ.fits (rows_tile * columns_tile)));
+  let nblk = rows_tile *^ columns_tile;
+
+  assume (pure (bdim * bdim < pow2 60)); // trivial
+  assert (pure (pow2 60 < pow2 64)); // trivial
+  assert (pure (SZ.fits (bdim * bdim)));
+  let nthr = bdim *^ bdim;
+  assert (pure (SZ.fits (nblk * nthr)));
   let size = nblk *^ nthr;
   let ar = Pulse.Lib.Array.alloc 0UL size;
 
-  let ga1 = gpu_array_alloc #u64 (Kernel.rows *^ Kernel.shared);
-  let ga2 = gpu_array_alloc #u64 (Kernel.shared *^ Kernel.columns);
+  assert (pure (SZ.fits (rows * shared)));
+  let ga1 = gpu_array_alloc #u64 (rows *^ shared);
+  assert (pure (SZ.fits (shared * columns)));
+  let ga2 = gpu_array_alloc #u64 (shared *^ columns);
 
-  GPU.Array.gpu_memcpy_host_to_device ga1 a1 (Kernel.rows *^ Kernel.shared);
-  GPU.Array.gpu_memcpy_host_to_device ga2 a2 (Kernel.shared *^ Kernel.columns);
+  GPU.Array.gpu_memcpy_host_to_device ga1 a1 (rows *^ shared);
+  GPU.Array.gpu_memcpy_host_to_device ga2 a2 (shared *^ columns);
 
   let gr = gpu_array_alloc #u64 size;
 
-  setup nblk nthr ga1 ga2 gr v1 v2;
+  let _ = calc (==) {
+    nblk * nthr;
+    == {}
+    ((rows / bdim) * (columns / bdim)) * (bdim * bdim);
+    == { magic() } // just associativity, sigh
+    (rows / bdim) * (columns / bdim) * bdim * bdim;
+    == { magic () } // fixme, boring proof (we have divisibility)
+    rows * columns;
+  };
+  assert (pure (nblk * nthr == rows * columns));
+
+  setup rows shared columns bdim (hide nblk) (hide nthr) ga1 ga2 gr v1 v2;
+ 
+  assume (pure (rows_tile * columns_tile <= rows * columns));
+
+  assume (pure (nblk <= max_threads)); // make sure to prove
+  assume (pure (nthr <= max_threads));
 
   let smem_sz = 2sz *^ nthr;
   launch_kernel_n_m_sync #0
     nblk
     nthr
-    #(fun (tid: nat {0 <= tid /\ tid < (nblk * nthr)} ) -> Kernel.kpre Kernel.rows Kernel.shared Kernel.columns ga1 ga2 gr #v1 #v2 (nblk * nthr) (Kernel.tid_to_idx tid))
-    #(fun (tid: nat {0 <= tid /\ tid < (nblk * nthr)} ) -> Kernel.kpost Kernel.rows Kernel.shared Kernel.columns ga1 ga2 gr #v1 #v2 (nblk * nthr) (Kernel.tid_to_idx tid))
+    #(fun (tid: nat {0 <= tid /\ tid < (nblk * nthr)} ) ->
+       Kernel.kpre rows shared columns ga1 ga2 gr #v1 #v2 (nblk * nthr)
+         (Kernel.tid_to_idx rows shared columns bdim tid))
+    #(fun (tid: nat {0 <= tid /\ tid < (nblk * nthr)} ) ->
+       Kernel.kpost rows shared columns ga1 ga2 gr #v1 #v2 (nblk * nthr)
+         (Kernel.tid_to_idx rows shared columns bdim tid))
     u64
     smem_sz
     #(Barrier.shared_pre nthr 0)
-    #(Barrier.shared_pre nthr (2 * Kernel.columns_tile))
+    #(Barrier.shared_pre nthr (2 * (shared / bdim)))
     (Barrier.block_setup_ghost nthr smem_sz)
-    (fun ear etid -> Kernel.kernel ga1 ga2 gr #v1 #v2 (hide nblk) (hide nthr) smem_sz ear etid);
+    (fun ear etid -> Kernel.kernel rows shared columns bdim ga1 ga2 gr #v1 #v2 (hide nblk) (hide nthr) smem_sz ear etid);
 
-  breakdown nblk nthr ga1 ga2 gr v1 v2;
+  breakdown rows shared columns bdim nblk nthr ga1 ga2 gr v1 v2;
 
   GPU.Array.gpu_memcpy_device_to_host ar gr size;
 
